Add solution for Pset7

pset7/Pset7.v
@@ -2,7 +2,878 @@
 
 Require Import Frap Pset7Sig.
 
+Ltac elimc var := elim var; clear var.
+Ltac pinvert expr := pose (pinvert_tmp := expr); invert pinvert_tmp.
+
+Lemma strong_induction0 {P: nat -> Prop} :
+    P O ->
+    (forall n:nat, n <> 0 -> (forall p:nat, p < n -> P p) -> P n) ->
+    forall n:nat, (forall p:nat, p < n -> P p).
+Proof.
+  intros P0 rec n; elimc n.
+  (* O *)
+    intros p absurd; discriminate (le_n_0_eq _ absurd).
+  (* S p *)
+    intros n H p Hp; induct Hp.
+      induct n; try exact P0. refine (rec (S n) _ H). discriminate.
+      exact (H p Hp).
+Qed.
+Theorem strong_induction {P: nat -> Prop} :
+    P O -> (forall n, n <> 0 -> (forall p, p < n -> P p) -> P n) ->
+    forall n, P n.
+Proof fun P0 rec n => strong_induction0 P0 rec (S n) n (le_n _).
+
+
+
+
+
+(* ========================= Map library extension ========================= *)
+
+
+Lemma includes_refl : forall {A B} (m:fmap A B), m $<= m.
+Proof.
+  intros A B m; refine (includes_intro _).
+  exact (fun _ _ H => H).
+Qed.
+
+Lemma includes_trans : forall {A B} (m1 m2 m3: fmap A B),
+    m1 $<= m2 -> m2 $<= m3 -> m1 $<= m3.
+Proof.
+  intros A B m1 m2 m3 H1 H2; refine (includes_intro _); intros k v H3.
+  exact (includes_lookup (includes_lookup H3 H1) H2).
+Qed.
+
+Lemma includes_nonexistent {A B} {m m' : fmap A B} {k} :
+    m $<= m' -> m' $? k = None -> m $? k = None.
+Proof.
+  intros H1 H2; cases (m $? k); try reflexivity.
+  rewrite (includes_lookup Heq H1) in H2; discriminate H2.
+Qed.
+
+Lemma includes_add_nonexistent {A B} {m m' : fmap A B} {k v} :
+    (forall (x y:A), sumbool (x=y) (x<>y)) ->
+    m $<= m' -> m $? k = None -> m $<= m' $+ (k, v).
+Proof.
+  intros A_dec m_le mk_none; refine (includes_intro _).
+  intros k0 v0 mk0.
+  cases (A_dec k0 k).
+    invert e; rewrite mk_none in mk0; discriminate mk0.
+    rewrite (lookup_add_ne _ _ n).
+    exact (includes_lookup mk0 m_le).
+Qed.
+
+(* Map Equality *)
+
+Definition map_eq {A B} (m m': fmap A B) : Prop :=
+    forall (x:A), m $? x = m' $? x.
+Infix "$==" := map_eq (at level 90).
+
+Lemma map_eq_refl : forall {A B} (m: fmap A B), m $== m.
+Proof fun A B m x => eq_refl (m $? x).
+Lemma map_eq_sym : forall {A B} {m m': fmap A B}, m $== m' -> m' $== m.
+Proof fun A B m m' H x => eq_sym (H x).
+Lemma map_eq_trans : forall {A B} {m1 m2 m3: fmap A B},
+    m1 $== m2 -> m2 $== m3 -> m1 $== m3.
+Proof fun A B m1 m2 m3 H1 H2 x => eq_trans (H1 x) (H2 x).
+
+Ltac map_rewritel Heq := refine (map_eq_trans Heq _).
+Ltac map_rewriter Heq := refine (map_eq_trans _ (map_eq_sym Heq)).
+
+(* Other properties *)
+
+Lemma plus_minus : forall {A B} (m: fmap A B) k v,
+    (forall x y:A, sumbool (x=y) (x<>y)) ->
+    m $+ (k, v) $- k $== m $- k.
+Proof.
+  intros A B m k1 v A_dec k2; cases (A_dec k2 k1).
+  (* k2 = k1 *)
+    repeat rewrite (lookup_remove_eq _ (eq_sym e)); reflexivity.
+  (* k2 <> k1 *)
+    repeat rewrite (lookup_remove_ne _ n).
+    rewrite (lookup_add_ne _ _ n); reflexivity.
+Qed.
+
+Lemma map_eq_leq {A B} (m m': fmap A B):
+    m $== m' <-> (m $<= m') /\ (m' $<= m).
+Proof.
+  split.
+  (* -> *)
+    intro H; split; refine (includes_intro _); intros k v H2;
+       [ pose (Heq := map_eq_sym H) | pose (Heq := H) ];
+       rewrite (Heq k); exact H2.
+  (* <- *)
+    intros [H1 H2] x; cases (m $? x).
+    (* Some b *)
+      exact (eq_sym (includes_lookup Heq H1)).
+    (* None *)
+      cases (m' $? x); try reflexivity.
+      rewrite (includes_lookup Heq0 H2) in Heq; discriminate Heq.
+Qed.
+
+Lemma map_eq_through_minus: forall {A B} {m m': fmap A B} k,
+    (forall x y:A, sumbool (x=y) (x<>y)) ->
+    m $== m' -> m $- k $== m' $- k.
+Proof.
+  intros A B m m' k1 A_dec H k2; cases (A_dec k2 k1).
+    repeat rewrite (lookup_remove_eq _ (eq_sym e)); reflexivity.
+    repeat rewrite (lookup_remove_ne _ n); exact (H k2).
+Qed.
+
+(* Map difference *)
+
+Definition map_diff {A B} (m m': fmap A B) : fmap A B :=
+    restrict (fun k => (m' $? k = None)) m.
+Infix "$--" := map_diff (at level 50, left associativity).
+
+Lemma diff_includes : forall {A B} (m m': fmap A B) k v,
+    (m $-- m') $? k = Some v -> m $? k = Some v.
+Proof.
+  intros A B m m' k v H.
+  rewrite <- (lookup_restrict_true _ m k (lookup_restrict_true_fwd H)).
+  exact H.
+Qed.
+
+Lemma option_none_dec : forall {B} (res: option B),
+    sumbool (res=None) (res<>None).
+Proof.
+  intros B res; cases res.
+    right; intro absurd; discriminate absurd.
+    left; reflexivity.
+Qed.
+Lemma diff_minus_assoc : forall {A B} (m1 m2: fmap A B) k,
+    (forall x y:A, sumbool (x=y) (x<>y)) ->
+    (m1 $-- m2) $- k $== (m1 $- k) $-- m2.
+Proof.
+  intros A B m1 m2 k1 A_dec k2; cases (A_dec k2 k1).
+  (* k1 = k2 *)
+    rewrite (lookup_remove_eq _ (eq_sym e)).
+    cases (option_none_dec (m2 $? k2)); unfold map_diff.
+    (* m2 $? k2 = None *)
+      rewrite (lookup_restrict_true _ _ k2 e0).
+      rewrite (lookup_remove_eq _ (eq_sym e)); reflexivity.
+    (* m2 $? k2 <> None *)
+      rewrite (lookup_restrict_false _ _ k2 n); reflexivity.
+  (* k1 <> k2 *)
+    rewrite (lookup_remove_ne _ n).
+    cases (option_none_dec (m2 $? k2)); unfold map_diff.
+    (* m2 $? k2 = None *)
+      repeat rewrite (lookup_restrict_true _ _ k2 e).
+      rewrite (lookup_remove_ne _ n); reflexivity.
+    (* m2 $? k2 <> None *)
+      repeat rewrite (lookup_restrict_false _ _ k2 n0); reflexivity.
+Qed.
+
+Lemma split_diff : forall {A B} (m1 m2: fmap A B) k v,
+    (forall x y:A, sumbool (x=y) (x<>y)) ->
+    m1 $-- (m2 $+ (k, v)) $== (m1 $-- m2) $- k.
+Proof.
+  intros A B m1 m2 k1 v A_dec k2; cases (A_dec k2 k1).
+  (* k1 <> k2 *)
+    rewrite (lookup_remove_eq _ (eq_sym e)).
+    cases (option_none_dec ((m2 $+ (k1, v)) $? k2)); unfold map_diff.
+    (* m1 $? k2 = None *)
+      rewrite (lookup_add_eq m2 v (eq_sym e)) in e0; discriminate e0.
+    (* m1 $? k2 <> None *)
+      rewrite (lookup_restrict_false _ _ k2 n); reflexivity.
+  (* k1 = k2 *)
+    rewrite (lookup_remove_ne _ n).
+    cases (option_none_dec ((m2 $+ (k1, v)) $? k2)); unfold map_diff.
+    (* (m2 $+ (k1, v)) $? k2 = None *)
+      rewrite (lookup_restrict_true _ _ k2 e).
+      rewrite (lookup_add_ne m2 v n) in e.
+      rewrite (lookup_restrict_true _ _ k2 e); reflexivity.
+    (* (m2 $+ (k1, v)) $? k2 <> None *)
+      rewrite (lookup_restrict_false _ _ k2 n0).
+      rewrite (lookup_add_ne m2 v n) in n0.
+      rewrite (lookup_restrict_false _ _ k2 n0); reflexivity.
+Qed.
+
+Lemma map_eq_through_diff : forall {A B} {m1 m2 m1' m2': fmap A B},
+    m1 $== m1' -> m2 $== m2' -> m1 $-- m2 $== m1' $-- m2'.
+Proof.
+  intros A B m1 m2 m1' m2' H1 H2 k.
+  cases (option_none_dec (m2 $? k)); unfold map_diff.
+  (* m2 $? k = None *)
+    rewrite (lookup_restrict_true _ m1 k e).
+    rewrite (H2 k) in e.
+    rewrite (lookup_restrict_true _ m1' k e).
+    rewrite (H1 k); reflexivity.
+  (* m2 $? k <> None *)
+    rewrite (lookup_restrict_false _ m1 k n).
+    rewrite (H2 k) in n.
+    rewrite (lookup_restrict_false _ m1' k n); reflexivity.
+Qed.
+
+Lemma diff_discard : forall {A B} (m1: fmap A B) {m2 k} v,
+    (forall x y:A, sumbool (x=y) (x<>y)) ->
+    m2 $? k <> None -> m1 $+ (k, v) $-- m2 $== m1 $-- m2.
+Proof.
+  intros A B m1 m2 k1 v A_dec H k2; cases (A_dec k2 k1); unfold map_diff.
+  (* k2 = k1 *)
+    rewrite <- e in H.
+    repeat rewrite (lookup_restrict_false _ _ k2 H); reflexivity.
+  (* k2 <> k1 *)
+    cases (option_none_dec (m2 $? k2)).
+      repeat rewrite (lookup_restrict_true _ _ k2 e);
+          rewrite (lookup_add_ne m1 v n); reflexivity.
+      repeat rewrite (lookup_restrict_false _ _ k2 n0); reflexivity.
+Qed.
+
+Lemma bigger_diff_eq {A B} {m1 m2 r1 r2: fmap A B} :
+    m1 $-- r1 $== m2 $-- r1 -> r1 $<= r2 -> m1 $-- r2 $== m2 $-- r2.
+Proof.
+  intros H1 H2 x.
+  cases (option_none_dec (r2 $? x)).
+  (* None *)
+    unfold map_diff; repeat rewrite
+        (lookup_restrict_true (fun k => (lookup r2 k = None)) _ _ e).
+    pose (H1x := H1 x).
+    unfold map_diff in H1x; repeat rewrite
+        (lookup_restrict_true (fun k => (lookup r1 k = None)) _ _
+          (includes_nonexistent H2 e)) in H1x.
+    exact H1x.
+  (* Some b *)
+    unfold map_diff; repeat rewrite
+        (lookup_restrict_false (fun k => (lookup r2 k = None)) _ _ n).
+    reflexivity.
+Qed.
+
+Lemma add_under_diff {A B} {m1 m2 r: fmap A B} k v :
+    (forall x y:A, sumbool (x=y) (x<>y)) ->
+    m1 $-- r $== m2 $-- r -> m1 $+ (k,v) $-- r $== m2 $+ (k,v) $-- r.
+Proof.
+  intros A_dec H x.
+  pose (Hx := H x); unfold map_diff; unfold map_diff in Hx.
+  cases (option_none_dec (r $? x)).
+  (* r $? x = None *)
+    repeat rewrite (lookup_restrict_true (fun k => (r $? k = None)) _ _ e).
+    repeat rewrite (lookup_restrict_true (fun k => (r $? k = None)) _ _ e)
+        in Hx.
+    cases (A_dec x k).
+      repeat rewrite (lookup_add_eq _ _ (eq_sym e0)); reflexivity.
+      repeat rewrite (lookup_add_ne _ _ n); exact Hx.
+  (* r $? x <> None *)
+    repeat rewrite (lookup_restrict_false (fun k => (r $? k = None)) _ _ n).
+    reflexivity.
+Qed.
+
+
+
+
+
+(* ============= Additional properties on Pset7Sig definitions ============== *)
+
+
+Lemma validator_on_same_cmds: forall {sc md1 md2},
+    validator' sc sc md1 = Some md2 -> md1 = md2.
+Proof.
+  intro sc; elimc sc; invert 1; try reflexivity.
+  (* Assign *)
+    cases (md1 $? x); cases (arithNotReading e md1);
+        cases (cmd_eq_dec (x <- e) (x <- e)); cases e; try discriminate H1;
+        invert H1; reflexivity.
+  (* Sequence *)
+    cases (validator' c1 c1 md1); cases (validator' c2 c2 md1);
+        try discriminate H3.
+      exact (eq_trans (H _ _ Heq) (H0 _ _ H3)).
+      rewrite (H _ _ Heq) in Heq0; rewrite H3 in Heq0; discriminate Heq0.
+  (* If *)
+    cases (validator' then_ then_ md1); cases (validator' else_ else_ md1);
+        cases (cmd_eq_dec (when e then then_ else else_ done)
+            (when e then then_ else else_ done));
+        cases (arithNotReading e md1 && cmdNotReading then_ md1 &&
+            cmdNotReading else_ md1); try discriminate H3.
+    invert H3; reflexivity.
+  (* While *)
+    cases (validator' body body md1); cases (arithNotReading e md1);
+        cases (cmd_eq_dec (while e loop body done) (while e loop body done));
+        try discriminate H2.
+    invert H2; reflexivity.
+  (* Output *)
+    cases (arith_eq_dec e e); cases (arithNotReading e md1);
+        try discriminate H1.
+    invert H1; reflexivity.
+Qed.
+
+Theorem validator_incr : forall {c1 c2 m1 m2},
+    validator' c1 c2 m1 = Some m2 -> m1 $<= m2.
+Proof.
+  intro c1; elim c1; clear c1.
+  (* Skip *)
+    intros c2 m1 m2 H; invert H; cases c2; try discriminate H1.
+    invert H1; exact (includes_refl m2).
+  (* Nop *)
+    intros c2 m1 m2 H; invert H; cases c2; try discriminate H1.
+    (* Nop Nop *)
+      invert H1; exact (includes_refl _).
+    (* Nop Assign *)
+      cases e; try discriminate H1.
+      cases (m1 $? x); try discriminate H1.
+      invert H1.
+      exact (includes_add_nonexistent string_dec (includes_refl m1) Heq).
+  (* Assign *)
+    intros v e c2 m1 m2 H; invert H; cases c2; try (cases e; discriminate H1).
+    (* Assign Nop *)
+      cases e; try discriminate H1.
+      cases (m1 $? v); try discriminate H1.
+      cases (n ==n n0); try discriminate H1.
+      invert H1; exact (includes_refl _).
+    (* Assign Assign *)
+      cases (cmd_eq_dec (v <- e) (x <- e0));
+          cases (arithNotReading e m1);
+          cases (m1 $? x);
+          try (cases e; discriminate H1).
+      cases e; invert H1; exact (includes_refl _).
+  (* Seq *)
+    intros ca reca cb recb c2 m1 m2 H; invert H; cases c2; try discriminate H1.
+    cases (validator' ca c2_1 m1); try discriminate H1.
+    exact (includes_trans m1 m m2 (reca _ _ _ Heq) (recb _ _ _ H1)).
+  (* If *)
+    intros e ca reca cb recb c2 m1 m2 H; invert H;
+        cases c2; try discriminate H1.
+    cases (validator' ca c2_1 m1); try discriminate H1.
+    cases (validator' cb c2_2 m1); try discriminate H1.
+    cases (cmd_eq_dec (when e then ca else cb done)
+                      (when e0 then c2_1 else c2_2 done)); try discriminate H1.
+    invert e1.
+    cases (arithNotReading e0 m1 && cmdNotReading c2_1 m1 &&
+           cmdNotReading c2_2 m1); try discriminate H1.
+    invert H1; exact (includes_refl _).
+  (* While *)
+    intros e c1 rec c2 m1 m2 H; invert H; cases c2; try discriminate H1.
+    cases (validator' c1 c2 m1); try discriminate H1.
+    cases (cmd_eq_dec (while e loop c1 done) (while e0 loop c2 done));
+        try discriminate H1.
+    cases (arithNotReading e m1); try discriminate H1.
+    invert H1; exact (includes_refl _).
+  (* Output *)
+    intros e c2 m1 m2 H; invert H; cases c2; try discriminate H1.
+    cases (arith_eq_dec e e0); try discriminate H1.
+    cases (arithNotReading e m1); try discriminate H1.
+    invert H1; exact (includes_refl _).
+Qed.
+
+Theorem arith_sub {e md v1 v2} :
+    arithNotReading e md = true -> v1 $-- md $== v2 $-- md ->
+    interp e v1 = interp e v2.
+Proof.
+  elimc e; try (* Const *) reflexivity; try ((* Plus, Minus, Times *)
+      intros e1 rec1 e2 rec2 H1 H2; simpl;
+      pinvert (proj1 (andb_true_iff _ _) H1);
+      rewrite (rec1 H H2); rewrite (rec2 H0 H2); reflexivity).
+  (* Var *)
+  intros x H1 H2. simpl. simpl in H1.
+  cases (md $? x); try discriminate H1.
+  pose (solution := H2 x).
+  unfold map_diff in solution.
+  repeat rewrite (lookup_restrict_true (fun k => (lookup md k = None)) _ x Heq)
+      in solution.
+  rewrite solution; reflexivity.
+Qed.
+
+
+
+
+
+(* =============================== Generation =============================== *)
+
+
+Inductive my_generate :
+    valuation * cmd -> list (option (option nat)) -> valuation -> Prop :=
+  | MyGenDone : forall v c,
+      my_generate (v, c) [] v
+  | MyGenSkip : forall v,
+      my_generate (v, Skip) [None] v
+  | MyGenStep : forall vc l vc' ns vf,
+      cstep vc l vc' ->
+      my_generate vc' ns vf ->
+      my_generate vc (Some l :: ns) vf.
+
+Lemma gen_unicity_n : forall {n vc l1 l2 vf1 vf2},
+    my_generate vc l1 vf1 -> my_generate vc l2 vf2 ->
+    length l1 = n -> length l2 = n -> l1 = l2 /\ vf1 = vf2.
+Proof.
+  intro n; elimc n.
+  (* O *)
+    intros vc l1 l2 vf1 vf2 H1 H2 l1len l2len.
+    pose (l1empty := proj1 (length_zero_iff_nil l1) l1len); invert l1empty.
+    pose (l2empty := proj1 (length_zero_iff_nil l2) l2len); invert l2empty.
+    induct H1; induct H2; exact (conj (eq_refl _) (eq_refl _)).
+  (* S n *)
+    intros n rec (v,c) l1 l2 vf1 vf2 H1 H2 l1slen l2slen.
+    induct l1; try discriminate l1slen; clear IHl1.
+    induct l2; try discriminate l2slen; clear IHl2.
+    assert (length l1 = n) as l1len; try exact (f_equal pred l1slen).
+    assert (length l2 = n) as l2len; try exact (f_equal pred l2slen).
+    induct H1.
+    (* MyGenSkip *)
+      invert l1slen; clear H0.
+      pose (l2empty := proj1 (length_zero_iff_nil l2) l2len); invert l2empty.
+      invert H2.
+        exact (conj (eq_refl _) (eq_refl _)).
+        invert H3; invert H1; invert H2.
+    (* MyGenStep *)
+      clear IHmy_generate.
+      induct H2; try (invert H; invert H3; invert H4); clear IHmy_generate.
+      pose (equalities := deterministic H0 H); destruct equalities, H3, H4.
+      pose (solution := rec _ _ _ _ _ H1 H2 l1len l2len); invert solution.
+      exact (conj (eq_refl _) (eq_refl _)).
+Qed.
+Theorem gen_unicity {vc l1 l2 vf1 vf2} :
+    my_generate vc l1 vf1 -> my_generate vc l2 vf2 -> length l1 = length l2 ->
+    l1 = l2 /\ vf1 = vf2.
+Proof fun H1 H2 leneq => gen_unicity_n H1 H2 leneq (eq_refl _).
+
+Theorem gen_prefix : forall {l1 vc l2 vf1 vf2},
+    my_generate vc l1 vf1 -> my_generate vc l2 vf2 ->
+    length l1 <= length l2 -> exists lq, l1 ++ lq = l2.
+Proof.
+  intro l1; elimc l1; try (
+      intros vc l2 vf1 vf2 _ _ _; exists l2; reflexivity).
+  intros a l1 rec vc l2 vf1 vf2 gen1 gen2 lencmp; invert gen1.
+  (* MyGenSkip *)
+    invert gen2; [invert lencmp | | invert H; invert H3; invert H4].
+    exists nil; reflexivity.
+  (* MyGenStep *)
+    invert gen2; [ invert lencmp | invert H2; invert H1; invert H3 |].
+    pinvert (deterministic H H2).
+    elim (rec vc' ns vf1 vf2 H4 H0 (le_S_n _ _ lencmp)).
+    intros lq Hrec; exists lq.
+    rewrite <- (app_comm_cons _ _ _); rewrite Hrec; reflexivity.
+Qed.
+
+Lemma split_gen : forall {vc l vc' l' ns vf},
+    cstep vc l vc' -> my_generate vc (Some l' :: ns) vf ->
+    l = l' /\ my_generate vc' ns vf.
+Proof.
+  intros vc l vc' l' ns vf step H; induct H.
+  pose (eqs := deterministic step H); invert eqs.
+  exact (conj (eq_refl _) H0).
+Qed.
+
+Lemma split_seq0: forall {n vi1 s1 s2 outs vf1},
+    my_generate (vi1, Sequence s1 s2) outs vf1 -> length outs = n
+    ->
+      my_generate (vi1, s1) outs vf1 /\ ~ In None outs
+      \/
+      exists outs1 outs2 vfmid1,
+        my_generate (vi1, s1) (outs1 ++ [None]) vfmid1
+        /\
+        my_generate (vfmid1, s2) (outs2) vf1
+        /\
+        outs = outs1 ++ [Some None] ++ outs2.
+Proof.
+  intro n; elimc n.
+  (* O *)
+    intros vi1 s1 s2 outs vf1 H no_outs.
+    pinvert (proj1 (length_zero_iff_nil _) no_outs); left.
+    invert H.
+    exact (conj (MyGenDone vf1 s1) (fun H => in_nil H)).
+  (* S n *)
+    intros n rec vi1 s1 s2 outs vf1 Hseq outs_len.
+    cases outs; try discriminate outs_len.
+    invert Hseq; invert H2; invert H1.
+    (* s1 stops *)
+      right; exists [], outs, vi1.
+      invert H3; invert H7.
+      exact (conj (MyGenSkip v') (conj H4 (eq_refl _))).
+    (* s1 continues *)
+      invert H7.
+      cases (rec v' c'0 s2 outs vf1 H4 (f_equal pred outs_len)).
+      (* s1 only *)
+        clear Heq; left; split.
+          exact (MyGenStep _ _ _ _ _ (CStep H5 H3 H6) (proj1 a)).
+          intro absurd; cases absurd; try discriminate; cases (proj2 a H).
+      (* s1 eventually stops *)
+        clear Heq; elimc e; intros outs1 tmp; elimc tmp; intros outs2 tmp.
+        elimc tmp; intros vfmid1 [midgen [finalgen outssum]].
+        right; exists (Some l::outs1), outs2, vfmid1.
+        repeat rewrite <- (app_comm_cons _ _ _); rewrite outssum.
+        exact (conj (MyGenStep _ _ _ _ _ (CStep H5 H3 H6) midgen)
+            (conj finalgen (eq_refl _))).
+Qed.
+Theorem split_seq {vi1 s1 s2 outs vf1} :
+    my_generate (vi1, Sequence s1 s2) outs vf1
+    ->
+      my_generate (vi1, s1) outs vf1 /\ ~ In None outs
+      \/
+      exists outs1 outs2 vfmid1,
+        my_generate (vi1, s1) (outs1 ++ [None]) vfmid1
+        /\
+        my_generate (vfmid1, s2) (outs2) vf1
+        /\
+        outs = outs1 ++ [Some None] ++ outs2.
+Proof fun H => split_seq0 H (eq_refl _).
+
+Lemma plug_step {vi c1 l vf c2} :
+    cstep (vi, c1) l (vf, c2) -> forall c3, cstep (vi, c1;; c3) l (vf, c2;; c3).
+Proof.
+  intros H c3; invert H.
+  exact (CStep (PlugSeq c3 H5) H6 (PlugSeq c3 H7)).
+Qed.
+Theorem plug_gen1 : forall {outs vi t1 vf},
+    my_generate (vi, t1) outs vf -> ~ In None outs ->
+    forall t2, my_generate (vi, t1;; t2) outs vf.
+Proof.
+  intro outs; elimc outs.
+  (* nil *)
+    intros vi t1 vf H _ t2; invert H.
+    exact (MyGenDone vf _).
+  (* a::outs *)
+    intros a outs rec vi t1 vf gen no_none t2; induct gen.
+    (* MyGenSkip *)
+      cases (no_none (or_introl (eq_refl None))).
+    (* MyGenStep *)
+      clear IHgen; induct vc'.
+      pose (no_none2 := fun H => no_none (in_cons (Some l) None outs H)).
+      exact (MyGenStep _ _ _ _ _ (plug_step H t2) (rec a b vf gen no_none2 t2)).
+Qed.
+
+Theorem plug_gen2 : forall {outs1 outs2 vi t1 t2 vm vf},
+    my_generate (vi, t1) (outs1 ++ [None]) vm ->
+    my_generate (vm, t2) outs2 vf ->
+    my_generate (vi, t1;; t2) (outs1 ++ [Some None] ++ outs2) vf.
+Proof.
+  intro outs1; elimc outs1.
+  (* nil *)
+    intros outs2 vi t1 t2 vm vf H1 H2; invert H1.
+    exact (MyGenStep _ _ _ _ _
+        (CStep (PlugHole _) (Step0Seq vm t2) (PlugHole _)) H2).
+  (* a::outs1 *)
+    intros a outs1 rec outs2 vi t1 t2 vm vf H1 H2; invert H1;
+        try cases (app_cons_not_nil _ _ _ H5).
+    induct vc'.
+    refine (MyGenStep _ _ _ _ _ _ (rec outs2 a b t2 vm vf H6 H2)).
+    exact (plug_step H4 t2).
+Qed.
+
+
+
+
+
+(* =============== Conclusion using simulation on valid_state =============== *)
+
+
+Definition valid_state (vc1 vc2: valuation * cmd) : Prop :=
+    forall ns vf1, my_generate vc1 ns vf1 ->
+    exists vf2, my_generate vc2 ns vf2.
+
+Theorem valid_state_refl : forall {vc1 vc2},
+    valid_state vc1 vc2 -> valid_state vc2 vc1.
+Proof.
+  assert (forall ns vc1 vc2 vf2, valid_state vc1 vc2 ->
+      my_generate vc2 ns vf2 ->
+      exists vf1, my_generate vc1 ns vf1) as reordered.
+    intro ns; elimc ns.
+    (* nil *)
+      exact (fun '(v,c) _ _ _ _ => ex_intro _ _ (MyGenDone v c)).
+    (* a::q *)
+      intros a q rec (v,c) vc2 vf2 H1 H2.
+      induct H2.
+      (* MyGenSkip *)
+        cases (skip_or_step v c).
+        (* Skip *)
+          clear Heq; invert e; exact (ex_intro _ _ (MyGenSkip v)).
+        (* CStep *)
+          clear Heq; elimc e; intros v' tmp; elimc tmp; intros l tmp; elimc tmp.
+          intros c' v0step.
+          elim (H1 [Some l] v' (MyGenStep _ _ _ _ _ v0step (MyGenDone _ _))).
+          intros vf2 vf2_gen.
+          discriminate (proj1 (gen_unicity vf2_gen (MyGenSkip v0) (eq_refl 1))).
+      (* MyGenStep *)
+        clear IHmy_generate.
+        cases (skip_or_step v c).
+        (* Skip *)
+          clear Heq; invert e; destruct vc.
+          pose (tmp := (H1 [None] v (MyGenSkip v))).
+          invert tmp; invert H0; invert H; invert H4; invert H5.
+        (* CStep *)
+          clear Heq; elimc e; intros v' tmp; elimc tmp.
+          intros l' tmp; elimc tmp; intros c' H'.
+          assert (valid_state (v', c') vc') as valid_followup.
+            intros ns vf1 Ha.
+            elim (H1 _ _ (MyGenStep _ _ _ _ _ H' Ha)); intros vf2 vf2_gen.
+            exact (ex_intro _ _ (proj2 (split_gen H vf2_gen))).
+          elim (H1 [Some l'] _ (MyGenStep _ _ _ _ _ H' (MyGenDone _ _))).
+          intros vf2 vf2_gen; induct vc'.
+          pose (l_eq_l' := proj1 (gen_unicity vf2_gen
+              (MyGenStep _ _ _ _ _ H (MyGenDone _ _)) (eq_refl 1))).
+          invert l_eq_l'.
+          elim (rec (v', c') (a, b) vf valid_followup H2).
+          intros vff vff_gen.
+          exact (ex_intro _ _ (MyGenStep _ _ _ _ _ H' vff_gen)).
+  exact (fun vc1 vc2 H ns vf2 => reordered ns vc1 vc2 vf2 H).
+Qed.
+
+Theorem validator_valid0 : forall s n t md1 md2,
+    validator' s t md1 = Some md2 ->
+    forall vi1 vi2,
+    (vi1 $-- md1) $== (vi2 $-- md1) ->
+    forall vf1 outs, my_generate (vi1, s) outs vf1 -> length outs = n ->
+    exists vf2,
+        my_generate (vi2, t) outs vf2
+        /\ ((vf1 $-- md2) $== (vf2 $-- md2)).
+Proof.
+  intro s; elimc s.
+  intros n t; cases t; try discriminate.
+  (* Skip Skip *)
+    intros md1 md2 valid vi1 vi2 vi12 vf1 outs gen1 outslen.
+    invert valid; invert gen1.
+      exact (ex_intro _ vi2 (conj (MyGenDone _ _) vi12)).
+      exact (ex_intro _ vi2 (conj (MyGenSkip _) vi12)).
+      invert H; invert H3; invert H4.
+  intros n t; cases t; try discriminate.
+  (* Nop Nop *)
+    intros md1 md2 valid vi1 vi2 vi12 vf1 outs gen1 outslen.
+    invert valid; invert gen1;
+        try exact (ex_intro _ vi2 (conj (MyGenDone _ _) vi12)).
+    invert H; invert H3; invert H4; invert H7.
+    pose (first_step := CStep (PlugHole _) (Step0Nop vi2) (PlugHole _)).
+    invert H0.
+      exact (ex_intro _ vi2
+          (conj (MyGenStep _ _ _ _ _ first_step (MyGenDone _ _)) vi12)).
+      exact (ex_intro _ vi2
+          (conj (MyGenStep _ _ _ _ _ first_step (MyGenSkip _)) vi12)).
+      invert H; invert H3; invert H4.
+  (* Nop, Assign x (Const n) *)
+    intros md1 md2 valid vi1 vi2 vi12 vf1 outs gen1 outslen.
+    simpl in valid.
+    cases e; cases (md1 $? x); try discriminate valid; invert valid.
+    pose (vi12x := (bigger_diff_eq vi12
+        (includes_add_nonexistent (v:=n0) string_dec (includes_refl _) Heq))).
+    invert gen1; try exact (ex_intro _ vi2 (conj (MyGenDone _ _) vi12x)).
+    invert H; invert H3; invert H4; invert H7.
+    pose (first_step := CStep (PlugHole _) (Step0Assign vi2 x n0) (PlugHole _)).
+    exists (vi2 $+ (x, interp n0 vi2)).
+    assert ((md1 $+ (x, n0)) $? x <> None) as x_discarded.
+      rewrite (lookup_add_eq _ _ (eq_refl _)); discriminate.
+    pose (vi12xx := map_eq_trans vi12x (map_eq_sym
+        (diff_discard _ (interp n0 vi2) string_dec x_discarded))).
+    invert H0.
+      exact (conj (MyGenStep _ _ _ _ _ first_step (MyGenDone _ _)) vi12xx).
+      exact (conj (MyGenStep _ _ _ _ _ first_step (MyGenSkip _)) vi12xx).
+      invert H; invert H3; invert H4.
+  intros x e n t; cases t; try (cases e; discriminate).
+  (* Assign x (Const n), Nop *)
+    intros md1 md2 valid vi1 vi2 vi12 vf1 outs gen1 outslen.
+    simpl in valid.
+    cases e; cases (md1 $? x); try discriminate valid.
+    cases (n0 ==n n1); try discriminate valid; invert valid.
+    invert gen1; try exact (ex_intro _ vi2 (conj (MyGenDone _ _) vi12)).
+    invert H; invert H3; invert H4; invert H7.
+    pose (first_step := CStep (PlugHole _) (Step0Nop vi2) (PlugHole _)).
+    assert (md2 $? x <> None) as md2_has_x; try (rewrite Heq; discriminate).
+    pose (vi12x := map_eq_trans (diff_discard _ n1 string_dec md2_has_x) vi12).
+    invert H0.
+      exact (ex_intro _ vi2
+          (conj (MyGenStep _ _ _ _ _ first_step (MyGenDone _ _)) vi12x)).
+      exact (ex_intro _ vi2
+          (conj (MyGenStep _ _ _ _ _ first_step (MyGenSkip _)) vi12x)).
+      invert H; invert H3; invert H4.
+  (* Assign sx se, Assign tx te *)
+    intros md1 md2 valid vi1 vi2 vi12 vf1 outs gen1 outslen.
+    simpl in valid.
+    cases (md1 $? x0); cases (cmd_eq_dec (x <- e) (x0 <- e0));
+        cases (arithNotReading e md1); try (cases e; discriminate valid).
+    assert (md1 = md2) as md12; try (cases e; invert valid; reflexivity).
+    invert md12; clear valid; invert e1.
+    invert gen1; try exact (ex_intro _ vi2 (conj (MyGenDone _ _) vi12)).
+    invert H; invert H3; invert H4; invert H7.
+    rewrite (arith_sub Heq0 vi12) in H0.
+    pose (vi12x0 := add_under_diff x0 (interp e0 vi2) string_dec vi12).
+    pose (first_step :=
+        CStep (PlugHole _) (Step0Assign vi2 x0 e0) (PlugHole _)).
+    exists (vi2 $+ (x0, interp e0 vi2)).
+    invert H0.
+      exact (conj (MyGenStep _ _ _ _ _ first_step (MyGenDone _ _)) vi12x0).
+      exact (conj (MyGenStep _ _ _ _ _ first_step (MyGenSkip _)) vi12x0).
+      invert H; invert H3; invert H4.
+  intros c1 rec1 c2 rec2 n t; cases t; try discriminate.
+  (* Sequence c1 c2, Sequence t1 t2 *)
+    intros md1 md2 valid vi1 vi2 vi12 vf1 outs gen1 outslen.
+    invert valid.
+    cases (validator' c1 t1 md1); try discriminate H0.
+    elim (split_seq gen1).
+    (* Case 1 *)
+      intros [gen11 no_none].
+      elim (rec1 _ _ _ _ Heq _ _ vi12 _ _ gen11 (eq_refl _)).
+      intros vf2 [gen21 vf12]; exists vf2.
+      exact (conj (plug_gen1 gen21 no_none t2)
+          (bigger_diff_eq vf12 (validator_incr H0))).
+    (* Case 2 *)
+      intro tmp; elimc tmp; intros outs1 tmp; elimc tmp; intros outs2 tmp;
+          elimc tmp; intros vfmid1 [gen3 [gen4 outsrel]].
+      elim (rec1 _ _ _ _ Heq _ _ vi12 _ _ gen3 (eq_refl _));
+          intros vfmid2 [gen6 eq6].
+      elim (rec2 _ _ _ _ H0 _ _ eq6 _ _ gen4 (eq_refl));
+          intros vf2 [gen7 eq7].
+      exists vf2; refine (conj _ eq7).
+      rewrite outsrel; exact (plug_gen2 gen6 gen7).
+  intros e c1 rec1 c2 rec2 n t; cases t; try discriminate.
+  (* If ..., If ... *)
+    intros md1 md2 valid vi1 vi2 vi12 vf1 outs gen1 outslen.
+    invert valid.
+    cases (validator' c1 t1 md1); cases (validator' c2 t2 md1);
+        cases (cmd_eq_dec (when e then c1 else c2 done)
+            (when e0 then t1 else t2 done));
+        cases (arithNotReading e md1 && cmdNotReading c1 md1 &&
+            cmdNotReading c2 md1);
+        try discriminate H0.
+    invert H0; invert e1.
+    pinvert (validator_on_same_cmds Heq).
+    pinvert (validator_on_same_cmds Heq0).
+    cases outs; invert gen1.
+    (* [] *)
+      exact (ex_intro _ vi2 (conj (MyGenDone vi2 _) vi12)).
+    (* Some l::outs *)
+      induct vc'.
+      pose (arith_e0 := proj1 (proj1 (andb_true_iff _ _)
+          (proj1 (proj1 (andb_true_iff _ _) Heq1)))).
+      invert H2; invert H6; invert H7; invert H8.
+      (* True *)
+        elim (rec1 _ _ _ _ Heq _ _ vi12 _ _ H4 (eq_refl _)).
+        intros vf2 [gen2 vf12]; exists vf2.
+        rewrite (arith_sub arith_e0 vi12) in H5.
+        pose (false_step :=
+            (CStep (PlugHole _) (Step0IfTrue vi2 e0 b t2 H5) (PlugHole _))).
+        exact (conj (MyGenStep _ _ _ _ _ false_step gen2) vf12).
+      (* False *)
+        elim (rec2 _ _ _ _ Heq0 _ _ vi12 _ _ H4 (eq_refl _)).
+        intros vf2 [gen2 vf12]; exists vf2.
+        rewrite (arith_sub arith_e0 vi12) in H5.
+        pose (false_step :=
+            (CStep (PlugHole _) (Step0IfFalse vi2 e0 t1 b H5) (PlugHole _))).
+        exact (conj (MyGenStep _ _ _ _ _ false_step gen2) vf12).
+  (* While ..., While ... *)
+    intros e c rec; refine (strong_induction _ _).
+    (* outs = [] *)
+      intro t; cases t; try discriminate.
+      intros md1 md2 valid vi1 vi2 vi12 vf1 outs gen1 outslen.
+      invert valid.
+      cases (validator' c t md1); cases (arithNotReading e md1);
+          cases (cmd_eq_dec (while e loop c done) (while e0 loop t done));
+          try discriminate H0.
+      invert H0; invert e1.
+      pinvert (validator_on_same_cmds Heq).
+      cases outs; try discriminate outslen.
+      induct gen1; exists vi2.
+      exact (conj (MyGenDone _ _) vi12).
+    (* Strong induction *)
+      intros n n_nonzero srec t; cases t; try discriminate.
+      intros md1 md2 valid vi1 vi2 vi12 vf1 outs gen1 outslen.
+      invert valid.
+      cases (validator' c t md1); cases (arithNotReading e md1);
+          cases (cmd_eq_dec (while e loop c done) (while e0 loop t done));
+          try discriminate H0.
+      invert H0; invert e1.
+      pinvert (validator_on_same_cmds Heq).
+      cases outs; try cases (n_nonzero (eq_refl O)); clear n_nonzero.
+      invert gen1; invert H2; invert H1; invert H7.
+      pinvert H3.
+      (* True *)
+        rewrite (arith_sub Heq0 vi12) in H5.
+        elim (split_seq H4).
+        (* t not completed *)
+          intros [gen1 no_none].
+          elim (rec _ _ _ _ Heq _ _ vi12 _ _ gen1 (eq_refl _)).
+          intros vf2 [gen2 vf12]; exists vf2.
+          exact (conj (MyGenStep _ _ _ _ _
+              (CStep (PlugHole _) (Step0WhileTrue vi2 e0 t H5) (PlugHole _))
+              (plug_gen1 gen2 no_none _)) vf12).
+        (* t completed *)
+          intro tmp; elimc tmp; intros outs1 tmp; elimc tmp; intros outs2 tmp;
+              elimc tmp; intros vfmid1 [gen3 [gen4 outsrel]].
+          elim (rec _ _ _ _ Heq _ _ vi12 _ _ gen3 (eq_refl _)).
+          intros vfmid2 [gen5 vfmid12].
+          assert (length outs2 < length (Some None :: outs)) as outs2sub.
+            simpl; rewrite outsrel; repeat rewrite (app_length _ _).
+            refine (le_n_S _ _ _); rewrite (plus_assoc _ _ _).
+            exact (le_plus_r _ _).
+          assert (validator' (while e0 loop t done) (while e0 loop t done) m
+              = Some m) as wvalid.
+            simpl; rewrite Heq; rewrite Heq0.
+            cases (cmd_eq_dec (while e0 loop t done) (while e0 loop t done));
+                [ reflexivity | cases (n (eq_refl _)) ].
+          elim (srec _ outs2sub _ _ _ wvalid _ _ vfmid12 _ _ gen4 (eq_refl _)).
+          intros vf2 [gen6 vf12]; exists vf2.
+          refine (conj (MyGenStep _ _ _ _ _
+              (CStep (PlugHole _) (Step0WhileTrue vi2 e0 t H5) (PlugHole _)) _)
+              vf12).
+          rewrite outsrel; exact (plug_gen2 gen5 gen6).
+      (* False *)
+        rewrite (arith_sub Heq0 vi12) in H5.
+        exists vi2; invert H4.
+        (* MyGenDone *)
+          exact (conj (MyGenStep _ _ _ _ _
+              (CStep (PlugHole _) (Step0WhileFalse vi2 e0 t H5) (PlugHole _))
+              (MyGenDone _ _)) vi12).
+        (* MyGenSkip *)
+          refine (conj (MyGenStep _ _ _ _ _
+              (CStep (PlugHole _) (Step0WhileFalse vi2 e0 t H5) (PlugHole _))
+              (MyGenSkip _)) vi12).
+        invert H; invert H4; invert H6.
+  intros e n t; cases t; try discriminate.
+  (* Output e, Output e0 *)
+    intros md1 md2 valid vi1 vi2 vi12 vf1 outs gen1 outslen; exists vi2.
+    simpl in valid; cases (arithNotReading e md1); cases (arith_eq_dec e e0);
+        try discriminate valid; invert valid.
+    invert gen1; try exact (conj (MyGenDone _ _) vi12).
+    invert H; invert H3; invert H4; invert H7.
+    rewrite (arith_sub Heq vi12).
+    pose (first_step := CStep (PlugHole _) (Step0Output vi2 e0) (PlugHole _)).
+    invert H0.
+      exact (conj (MyGenStep _ _ _ _ _ first_step (MyGenDone _ _)) vi12).
+      exact (conj (MyGenStep _ _ _ _ _ first_step (MyGenSkip _)) vi12).
+      invert H; invert H3; invert H4.
+Qed.
+
+Theorem validator_valid : forall s t v,
+    validator s t = true -> valid_state (v, s) (v, t).
+Proof.
+  intros s t v valid ns vf1 H; unfold validator in valid.
+  cases (validator' s t $0); try discriminate valid; clear valid.
+  elim (validator_valid0
+      s _ t $0 m Heq v v (map_eq_refl _) vf1 ns H (eq_refl _)).
+  intros vf2 [solution _]; exact (ex_intro _ vf2 solution).
+Qed.
+
+Lemma one_step_proof :
+    forall vc1 vc2,
+      valid_state vc1 vc2 -> forall vc1' l,
+        cstep vc1 l vc1' ->
+        exists vc2', cstep vc2 l vc2' /\ valid_state vc1' vc2'.
+Proof.
+  intros vc1 vc2 H1 vc1' l H2; destruct vc2.
+  cases (skip_or_step v c); induct vc1'.
+  (* Skip *)
+    clear Heq; invert e.
+    elim (valid_state_refl H1 [None] v (MyGenSkip v)); intros vf vc1_gen_none.
+    discriminate (proj1 (gen_unicity vc1_gen_none
+        (MyGenStep _ _ _ _ _ H2 (MyGenDone _ _)) (eq_refl 1))).
+  (* Step *)
+    clear Heq; elimc e; intros v' tmp; elimc tmp; intros l' tmp; elimc tmp.
+    intros c' vstep.
+    assert (l = l') as l_eq_l'.
+      elim (H1 [Some l] _ (MyGenStep _ _ _ _ _ H2 (MyGenDone _ _))).
+      intros vf vf_gen.
+      pose (l_eq_l' := proj1 (gen_unicity vf_gen
+          (MyGenStep _ _ _ _ _ vstep (MyGenDone _ _)) (eq_refl 1))).
+      invert l_eq_l'; reflexivity.
+    invert l_eq_l'; exists (v', c'); refine (conj vstep _).
+    intros ns vf Hns.
+    elim (H1 _ _ (MyGenStep _ _ _ _ _ H2 Hns)); intros vf2 vf2_gen.
+    exact (ex_intro _ _ (proj2 (split_gen vstep vf2_gen))).
+Qed.
+
+Lemma agree_on_termination_proof :
+    forall v1 v2 c2, valid_state (v1, Skip) (v2, c2) -> c2 = Skip.
+Proof.
+  intros v1 v2 c2 H; elim (H _ _ (MyGenSkip v1)).
+  intros vf gen2; invert gen2; reflexivity.
+Qed.
+
 Theorem validator_ok:
   forall v s t, validator s t = true -> (v, s) =| (v, t).
-Proof.
-Admitted.
+Proof fun v s t H => simulation
+    valid_state one_step_proof agree_on_termination_proof (v,s) (v,t)
+    (validator_valid s t v H).
